theories/Symbolic/PartialEvaluation.v
@@ -197,6 +197,12 @@ Module Type PartialEvaluationOn
       | None   => term_truncate m t
       end.
 
+    Definition peval_extract {n} (s l : nat) (t : Term Σ (ty.bvec n)) : Term Σ (ty.bvec l) :=
+      match term_get_val t with
+      | Some v => term_val (ty.bvec l) (bv.extract s l v)
+      | None   => term_extract s l t
+      end.
+
     Definition peval_union {U K} (t : Term Σ (unionk_ty U K)) : Term Σ (ty.union U) :=
       match term_get_val t with
       | Some v => term_val (ty.union U) (unionv_fold U (existT K v))
@@ -232,6 +238,7 @@ Module Type PartialEvaluationOn
       | term_get_slice_int t => peval_get_slice_int (peval t)
       | term_unsigned t     => peval_unsigned (peval t)
       | term_truncate m t   => peval_truncate m (peval t)
+      | term_extract s l t  => peval_extract s l (peval t)
       | term_tuple ts       => term_tuple (env.map (fun b => @peval b) ts)
       | term_union U K t    => peval_union (peval t)
       | term_record R ts    => peval_record R (env.map (fun b => peval (σ := type b)) ts)
@@ -273,6 +280,10 @@ Module Type PartialEvaluationOn
       @peval_truncate n m p t ≡ term_truncate m t.
     Proof. unfold peval_truncate; destruct (term_get_val_spec t); now subst. Qed.
 
+    Lemma peval_extract_sound {n} (s l : nat) (t : Term Σ (ty.bvec n)) :
+      @peval_extract n s l t ≡ term_extract s l t.
+    Proof. unfold peval_extract; destruct (term_get_val_spec t); now subst. Qed.
+
     Lemma peval_union_sound {U K} (t : Term Σ (unionk_ty U K)) :
       peval_union t ≡ term_union U K t.
     Proof. unfold peval_union. destruct (term_get_val_spec t); now subst. Qed.
@@ -312,6 +323,7 @@ Module Type PartialEvaluationOn
       - etransitivity; [apply peval_get_slice_int_sound |now apply proper_term_get_slice_int].
       - etransitivity; [apply peval_unsigned_sound |now apply proper_term_unsigned].
       - etransitivity; [apply peval_truncate_sound |now apply proper_term_truncate].
+      - etransitivity; [apply peval_extract_sound |now apply proper_term_extract].
       - apply proper_term_tuple.
         induction IH; [reflexivity|]; cbn.
         now apply proper_env_snoc.
