theories/Symbolic/Instantiation.v
@@ -117,6 +117,7 @@ Module Type InstantiationOn
     | term_get_slice_int t => bv.of_Z (inst (Inst := inst_term) t ι)
     | term_unsigned t      => bv.unsigned (inst (Inst := inst_term) t ι)
     | term_truncate m t    => bv.truncate m (inst (Inst := inst_term) t ι)
+    | term_extract s l t   => bv.extract s l (inst (Inst := inst_term) t ι)
     | @term_tuple _ σs ts  =>
         envrec.of_env (inst (Inst := inst_env (InstSA := @inst_term)) ts ι)
     | @term_union _ U K t     => unionv_fold U (existT K (inst (Inst := inst_term) t ι))
@@ -430,6 +431,7 @@ Module Type InstantiationOn
     #[export,program] Instance proper_term_get_slice_int {Σ n} : Proper ((≡) ==> (≡)) (@term_get_slice_int Σ n).
     #[export,program] Instance proper_term_unsigned {Σ n} : Proper ((≡) ==> (≡)) (@term_unsigned Σ n).
     #[export,program] Instance proper_term_truncate {Σ n m p} : Proper ((≡) ==> (≡)) (@term_truncate Σ n m p).
+    #[export,program] Instance proper_term_extract {Σ n s l} : Proper ((≡) ==> (≡)) (@term_extract Σ n s l).
     #[export,program] Instance proper_term_tuple {Σ σs} : Proper ((≡) ==> (≡)) (@term_tuple Σ σs).
     #[export,program] Instance proper_term_union {Σ U K} : Proper ((≡) ==> (≡)) (@term_union Σ U K).
     #[export,program] Instance proper_term_record {Σ R} : Proper ((≡) ==> (≡)) (@term_record Σ R).
